Prove LogAllEntries

raft-proofs/LogAllEntriesProof.v
@@ -15,6 +15,7 @@ Require Import RefinementSpecLemmas.
 Require Import UpdateLemmas.
 Local Arguments update {_} {_} {_} _ _ _ _ : simpl never.
 
+Require Import TermSanityInterface.
 Require Import LogAllEntriesInterface.
 
 Section LogAllEntries.
@@ -23,7 +24,272 @@ Section LogAllEntries.
   Context {raft_params : RaftParams orig_base_params}.
 
   Context {rri : raft_refinement_interface}.
+  Context {tsi : term_sanity_interface}.
 
+  Ltac update_destruct :=
+    match goal with
+      | [ |- context [ update _ ?y _ ?x ] ] => destruct (name_eq_dec y x)
+    end.
+
+  Ltac update_destruct_hyp :=
+    match goal with
+      | [ _ : context [ update _ ?y _ ?x ] |- _ ] => destruct (name_eq_dec y x)
+    end.
+
+  Ltac destruct_update :=
+    repeat (first [update_destruct_hyp|update_destruct]; subst; rewrite_update).
+
+  Ltac rewrite_goal :=
+    match goal with
+      | H: _ = _ |- _ => rewrite H
+    end.
+    
+  Definition no_entries_past_current_term_host_lifted net :=
+    forall (h : name) e,
+      In e (log (snd (nwState net h))) ->
+      eTerm e <= currentTerm (snd (nwState net h)).
+
+  Lemma no_entries_past_current_term_host_lifted_invariant :
+    forall net,
+      refined_raft_intermediate_reachable net ->
+      no_entries_past_current_term_host_lifted net.
+  Proof.
+    unfold no_entries_past_current_term_host_lifted.
+    pose proof deghost_spec.
+    do 4 intro.
+    repeat find_reverse_higher_order_rewrite.
+    eapply lift_prop; eauto.
+    intros.
+    find_apply_lem_hyp no_entries_past_current_term_invariant; eauto.
+  Qed.
+
+  Lemma handleAppendEntries_currentTerm_monotonic:
+    forall h st (d : raft_data) 
+      (m : msg) (t : term) (n : name) (pli : logIndex) 
+      (plt : term) (es : list entry) (ci : logIndex),
+      handleAppendEntries h st t n pli plt es
+                          ci = (d, m) ->
+      currentTerm st <= currentTerm d.
+  Proof.
+    intros.
+    unfold handleAppendEntries in *.
+    repeat break_match; simpl in *; do_bool; repeat find_inversion; auto; try omega;
+    simpl in *;
+    unfold advanceCurrentTerm in *; repeat break_match; do_bool; auto.
+  Qed.
+  
+  Lemma log_all_entries_append_entries :
+    refined_raft_net_invariant_append_entries log_all_entries.
+  Proof.
+    red. unfold log_all_entries. intros.
+    simpl in *. repeat find_higher_order_rewrite.
+    destruct_update; simpl in *; eauto;
+    [|copy_eapply_prop_hyp In In; repeat find_rewrite; auto].
+    find_copy_apply_lem_hyp handleAppendEntries_currentTerm_monotonic.
+    find_eapply_lem_hyp update_elections_data_appendEntries_log_allEntries;
+      intuition; eauto; repeat find_rewrite; repeat rewrite_goal; eauto.
+    - copy_eapply_prop_hyp In In; repeat find_rewrite; auto.
+      find_apply_lem_hyp no_entries_past_current_term_host_lifted_invariant; auto.
+      repeat find_rewrite. eauto using le_antisym.
+    - subst.
+      apply in_app_iff. right.
+      find_apply_hyp_hyp.
+      find_apply_lem_hyp no_entries_past_current_term_host_lifted_invariant; auto.
+      eauto using le_antisym.
+    - subst.
+      apply in_app_iff.
+      left.
+      apply in_map_iff. eauto.
+    - do_in_app. intuition.
+      + subst.
+        apply in_app_iff.
+        left.
+        apply in_map_iff. eauto.
+      + subst.
+        apply in_app_iff. right.
+        find_apply_lem_hyp removeAfterIndex_in.
+        find_apply_hyp_hyp.
+        find_apply_lem_hyp no_entries_past_current_term_host_lifted_invariant; auto.
+        eauto using le_antisym.
+  Qed.
+
+  Lemma log_all_entries_append_entries_reply :
+    refined_raft_net_invariant_append_entries_reply log_all_entries.
+  Proof.
+    red. unfold log_all_entries. intros.
+    simpl in *. repeat find_higher_order_rewrite.
+    destruct_update; simpl in *; eauto;
+    [|copy_eapply_prop_hyp In In; repeat find_rewrite; auto].
+    find_copy_apply_lem_hyp handleAppendEntriesReply_log. find_rewrite.
+    find_copy_apply_lem_hyp handleAppendEntriesReply_type_term.
+    intuition; repeat find_rewrite; copy_eapply_prop_hyp In In; repeat find_rewrite; auto.
+    find_apply_lem_hyp no_entries_past_current_term_host_lifted_invariant; auto.
+    repeat find_rewrite. eauto using le_antisym.
+  Qed.
+
+  Lemma log_all_entries_request_vote :
+    refined_raft_net_invariant_request_vote log_all_entries.
+  Proof.
+    red. unfold log_all_entries. intros.
+    simpl in *. repeat find_higher_order_rewrite.
+    destruct_update; simpl in *; eauto;
+    [|copy_eapply_prop_hyp In In; repeat find_rewrite; auto].
+    find_copy_apply_lem_hyp handleRequestVote_log. find_rewrite.
+    find_copy_apply_lem_hyp handleRequestVote_type_term.
+    rewrite update_elections_data_requestVote_allEntries.
+    intuition; repeat find_rewrite; copy_eapply_prop_hyp In In; repeat find_rewrite; auto.
+    find_apply_lem_hyp no_entries_past_current_term_host_lifted_invariant; auto.
+    repeat find_rewrite. eauto using le_antisym.
+  Qed.
+
+
+  Lemma log_all_entries_request_vote_reply :
+    refined_raft_net_invariant_request_vote_reply log_all_entries.
+  Proof.
+    red. unfold log_all_entries. intros.
+    simpl in *. repeat find_higher_order_rewrite.
+    destruct_update; simpl in *; eauto;
+    [|copy_eapply_prop_hyp In In; repeat find_rewrite; auto].
+    find_erewrite_lem handleRequestVoteReply_log.
+    rewrite update_elections_data_requestVoteReply_allEntries.
+    match goal with
+      | |- context [handleRequestVoteReply ?h ?st ?h' ?t ?v] =>
+        pose proof handleRequestVoteReply_type h st h' t v
+             (handleRequestVoteReply h st h' t v)
+    end.
+    intuition; repeat find_rewrite;
+    copy_eapply_prop_hyp In In; repeat find_rewrite; auto.
+    find_apply_lem_hyp no_entries_past_current_term_host_lifted_invariant; auto.
+    repeat find_rewrite.
+    unfold raft_data in *. simpl in *. 
+    unfold raft_data in *. simpl in *.
+    omega.
+  Qed.
+
+  Lemma log_all_entries_do_leader :
+    refined_raft_net_invariant_do_leader log_all_entries.
+  Proof.
+    red. unfold log_all_entries. intros.
+    match goal with
+      | H : nwState ?net ?h = (?gd, ?d) |- _ =>
+        replace gd with (fst (nwState net h)) in * by (rewrite H; reflexivity);
+          replace d with (snd (nwState net h)) in * by (rewrite H; reflexivity);
+          clear H
+    end.
+    simpl in *. repeat find_higher_order_rewrite.
+    destruct_update; simpl in *; eauto;
+    [|copy_eapply_prop_hyp In In; repeat find_rewrite; auto].
+    find_copy_apply_lem_hyp doLeader_type; intuition.
+    find_apply_lem_hyp doLeader_log. repeat find_rewrite.
+    copy_eapply_prop_hyp In In; repeat find_rewrite; auto.
+  Qed.
+  
+
+  Lemma log_all_entries_do_generic_server :
+    refined_raft_net_invariant_do_generic_server log_all_entries.
+  Proof.
+    red. unfold log_all_entries. intros.
+    match goal with
+      | H : nwState ?net ?h = (?gd, ?d) |- _ =>
+        replace gd with (fst (nwState net h)) in * by (rewrite H; reflexivity);
+          replace d with (snd (nwState net h)) in * by (rewrite H; reflexivity);
+          clear H
+    end.
+    simpl in *. repeat find_higher_order_rewrite.
+    destruct_update; simpl in *; eauto;
+    [|copy_eapply_prop_hyp In In; repeat find_rewrite; auto].
+    find_copy_apply_lem_hyp doGenericServer_type; intuition.
+    find_apply_lem_hyp doGenericServer_log. repeat find_rewrite.
+    copy_eapply_prop_hyp In In; repeat find_rewrite; auto.
+  Qed.
+
+  Lemma log_all_entries_client_request :
+    refined_raft_net_invariant_client_request log_all_entries.
+  Proof.
+    red. unfold log_all_entries. intros.
+    simpl in *. repeat find_higher_order_rewrite.
+    destruct_update; simpl in *; eauto;
+    [|copy_eapply_prop_hyp In In; repeat find_rewrite; auto].
+    find_copy_apply_lem_hyp update_elections_data_client_request_log_allEntries.
+    find_apply_lem_hyp handleClientRequest_type.
+    intuition; repeat find_rewrite;
+    [copy_eapply_prop_hyp In In; repeat find_rewrite; auto|].
+    break_exists. intuition.
+    repeat find_rewrite.  simpl in *. intuition; subst; auto.
+    copy_eapply_prop_hyp In In; repeat find_rewrite; auto.
+  Qed.
+
+  Lemma log_all_entries_timeout :
+    refined_raft_net_invariant_timeout log_all_entries.
+  Proof.
+    red. unfold log_all_entries. intros.
+    simpl in *. repeat find_higher_order_rewrite.
+    destruct_update; simpl in *; eauto;
+    [|copy_eapply_prop_hyp In In; repeat find_rewrite; auto].
+    find_copy_apply_lem_hyp handleTimeout_log_same.
+    rewrite update_elections_data_timeout_allEntries.
+    find_apply_lem_hyp handleTimeout_type_strong.
+    intuition; repeat find_rewrite;
+    copy_eapply_prop_hyp In In; repeat find_rewrite; auto.
+    find_apply_lem_hyp no_entries_past_current_term_host_lifted_invariant; auto.
+    repeat find_rewrite.
+    unfold raft_data in *. simpl in *. 
+    unfold raft_data in *. simpl in *.
+    omega.
+  Qed.
+
+  Lemma log_all_entries_reboot :
+    refined_raft_net_invariant_reboot log_all_entries.
+  Proof.
+    red. unfold log_all_entries. intros.
+    match goal with
+      | H : nwState ?net ?h = (?gd, ?d) |- _ =>
+        replace gd with (fst (nwState net h)) in * by (rewrite H; reflexivity);
+          replace d with (snd (nwState net h)) in * by (rewrite H; reflexivity);
+          clear H
+    end.
+    simpl in *. repeat find_higher_order_rewrite.
+    destruct_update; simpl in *; eauto;
+    copy_eapply_prop_hyp In In; repeat find_rewrite; auto.
+  Qed.
+
+  Lemma log_all_entries_init :
+    refined_raft_net_invariant_init log_all_entries.
+  Proof.
+    red. unfold log_all_entries. intros.
+    simpl in *. intuition.
+  Qed.
+
+  Lemma log_all_entries_state_same_packet_subset :
+    refined_raft_net_invariant_state_same_packet_subset log_all_entries.
+  Proof.
+    red. unfold log_all_entries. intros.
+    simpl in *.
+    repeat find_reverse_higher_order_rewrite.
+    copy_eapply_prop_hyp In In; repeat find_rewrite; auto.
+  Qed.
+
+  Theorem log_all_entries_invariant :
+    forall net,
+      refined_raft_intermediate_reachable net ->
+      log_all_entries net.
+  Proof.
+    intros. apply refined_raft_net_invariant; auto.
+    - apply log_all_entries_init.
+    - apply log_all_entries_client_request.
+    - apply log_all_entries_timeout.
+    - apply log_all_entries_append_entries.
+    - apply log_all_entries_append_entries_reply.
+    - apply log_all_entries_request_vote.
+    - apply log_all_entries_request_vote_reply.
+    - apply log_all_entries_do_leader.
+    - apply log_all_entries_do_generic_server.
+    - apply log_all_entries_state_same_packet_subset.
+    - apply log_all_entries_reboot.
+  Qed.
+  
   Instance laei : log_all_entries_interface.
-  Admitted.
+  split.
+  auto using log_all_entries_invariant.
+  Qed.
 End LogAllEntries.
